theories/prob_eff_lang/probblaze/pure_weakestpre.v
@@ -1,0 +1,48 @@
+From clutch.prob_eff_lang.probblaze Require Import primitive_laws.
+From iris.proofmode Require Import base proofmode.
+From clutch.prob_eff_lang.probblaze Require Import syntax semantics notation class_instances logic.
+
+(* Consider generalizing the PureExec construction *)
+Definition prel `{Σ : gFunctors} (e1 e2 : expr) (Φ : val → val → iProp Σ) : iProp Σ := 
+  match (to_val e1), (to_val e2) with
+  | Some v1, Some v2 => Φ v1 v2
+  | Some v1, None => ∃ (v2 : val) n2 Ψ2, ⌜Ψ2 ∧ PureExec Ψ2 n2 e2 v2⌝ ∗ Φ v1 v2
+  | None, Some v2 =>  ∃ (v1 : val) n1 Ψ1, ⌜Ψ1 ∧ PureExec Ψ1 n1 e1 v1⌝ ∗ Φ v1 v2
+  | None, None => ∃ (v1 v2 : val) n1 n2 Ψ1 Ψ2,  ⌜Ψ1 ∧ PureExec Ψ1 n1 e1 v1 ∧ Ψ2 ∧ PureExec Ψ2 n2 e2 v2⌝ ∗ Φ v1 v2
+  end. 
+
+Lemma prel_intuitionistically `{Σ : gFunctors} e1 e2 Φ : 
+  (□ prel e1 e2 Φ) -∗ @prel Σ e1 e2 (λ v1 v2, □ (Φ v1 v2)).
+Proof.
+  iIntros "#Hrel". unfold prel.
+  destruct (to_val e1) eqn:Heq1, (to_val e2) eqn:Heq2; first done.
+  1, 2: iDestruct "Hrel" as (???) "H"; iExists _,_; iDestruct "H" as "($ & H2)"; by iModIntro. 
+  iDestruct "Hrel" as (??????) "H". iExists _,_,_,_. iDestruct "H" as "($ & H2)". by iModIntro. 
+Qed. 
+
+Notation "'PREL' e1 ≤ e2 '[{' Φ '}]'" := (prel e1%E e2%E Φ)
+                                           (at level 20, e1, e2, Φ at next level, only parsing) : bi_scope.
+Lemma prel_brel `{!probblazeRGS Σ} e1 e2 Φ :                         
+  prel e1 e2 Φ -∗ brel ⊤ e1 e2 ⊥ Φ.
+Proof. 
+  iIntros "He". 
+  destruct (to_val e1) eqn:Heq1, (to_val e2) eqn:Heq2; rewrite /prel Heq1 Heq2/=.
+  - rewrite -(of_to_val _ _ Heq1). rewrite -(of_to_val _ _ Heq2). iApply brel_value. by iIntros "$ !>".
+  - rewrite -(of_to_val _ _ Heq1). iDestruct "He" as (???(?&?)) "HΦ".
+    iApply brel_pure_step_r; first done. iApply brel_value. by iIntros "$ !>".
+  - rewrite -(of_to_val _ _ Heq2). iDestruct "He" as (???(?&?)) "HΦ".
+    iApply brel_pure_step_later; first done. iApply brel_value. by iIntros "!> $ !>".
+  - iDestruct "He" as (??????(?&?&?&?)) "H". iApply brel_pure_step_r; first done.
+    iApply brel_pure_step_later; first done. iApply brel_value.
+    by iIntros "!> $ !>".
+Qed. 
+
+Lemma prel_mono `{Σ : gFunctors} e1 e2 Φ Ψ : 
+  (∀ v1 v2, Φ v1 v2 -∗ Ψ v1 v2) -∗
+  PREL e1 ≤ e2 [{ Φ }] -∗ @prel Σ e1 e2 Ψ.
+Proof.
+  iIntros "Hvv Hprel". rewrite /prel.
+  destruct (to_val e1) eqn:Heq1, (to_val e2) eqn:Heq2; [by iApply "Hvv" | | |].
+  1,2: iDestruct "Hprel" as (???) "($ & H)"; by iApply "Hvv".
+  iDestruct "Hprel" as (??????) "($ & H)"; by iApply "Hvv".
+Qed.
